adding call stack limit for stack exhaustion tests

src/execute.ml
@@ -54,22 +54,28 @@ type eval_cfg_result =
   | Cfg_err
   | Cfg_exhaustion
 
-let rec eval_interp_cfg verbosity gen fuel cfg =
+let rec eval_interp_cfg verbosity gen max_call_depth cfg d =
   let print_step_header gen =
     debug_info verbosity intermediate ~style:bold
       (fun () -> Printf.sprintf "step %d:\n" gen) in
-  if (fuel >= 0) && (gen >= fuel) then begin
+  if (max_call_depth >= 0) && (gen >= max_call_depth) then begin
     debug_info verbosity stage ~style:red (fun _ -> "Fuel exhaustion\n");
     Cfg_exhaustion
   end
   else
-    let cfg_res = run_one_step cfg in
+    let cfg_res = run_one_step cfg d in
       print_step_header gen;
       debug_info verbosity intermediate
         (fun _ -> pp_res_cfg_except_store cfg cfg_res);
       match cfg_res with
-      | RSC_normal (_hs', cfg') ->
-        eval_interp_cfg verbosity (gen+1) fuel cfg'
+      | RSC_normal (_hs', cfg', d') ->
+        let d_int = Convert.from_n d' in
+        if (d_int > max_call_depth) && (max_call_depth != -1) then begin
+          debug_info verbosity stage ~style:red (fun _ -> "Call stack exhaustion\n");
+          Cfg_exhaustion
+        end
+        else
+          eval_interp_cfg verbosity (gen+1) max_call_depth cfg' d_int
       | RSC_value (s, f, vs) ->
         debug_info verbosity stage ~style:green (fun _ -> "success after " ^ string_of_int gen ^ " steps\n");
         (Cfg_res (s, f, vs))
@@ -83,11 +89,11 @@ let rec eval_interp_cfg verbosity gen fuel cfg =
         debug_info verbosity stage ~style:red (fun _ -> "Ill-typed input\n");
         Cfg_err
   
-let eval_wasm_cfg verbosity fuel cfg =
+let eval_wasm_cfg verbosity max_call_depth cfg =
   let interp_cfg_inst = interp_cfg_of_wasm cfg in
   debug_info verbosity intermediate (fun _ ->
     Printf.sprintf "\nExecuting configuration:\n%s\n" (pp_cfg_tuple_ctx_except_store interp_cfg_inst));
-  eval_interp_cfg verbosity 1 fuel interp_cfg_inst
+  eval_interp_cfg verbosity 1 max_call_depth interp_cfg_inst 0
 
 
 module StringMap = Map.Make(String);;
@@ -108,7 +114,7 @@ let global_get verbosity hs s modname extname =
     end
   | None -> TopHost.error "Module not found"
 
-let invoke_func verbosity hs sf args modname name fuel =
+let invoke_func verbosity hs sf args modname name max_call_depth =
   let (exts, _) = hs in
   let (s, f) = sf in
   let* es_init =
@@ -128,7 +134,7 @@ let invoke_func verbosity hs sf args modname name fuel =
         end
       )) in
     let cfg_init = (s, (f, es_init)) in
-    pure (eval_wasm_cfg verbosity fuel cfg_init)
+    pure (eval_wasm_cfg verbosity max_call_depth cfg_init)
 
 let print_invoke_result verbosity res = 
   debug_info verbosity result (fun _ ->
