src/wast_execute.ml
@@ -171,13 +171,13 @@ let print_wast_command cmd =
 let wasm_name_to_raw_string n = 
   Wasm.Utf8.encode n
 
-let run_invoke verbosity act_invoke hs s default_module_name fuel = 
+let run_invoke verbosity act_invoke hs s default_module_name max_call_depth = 
   match act_invoke with
   | (ovar, funcname_utf8, val_args) ->
     let* modname = ovar_to_name default_module_name hs ovar in
     let funcname = wasm_name_to_raw_string funcname_utf8 in 
     let* args = wasm_vals_to_coq val_args in
-    let* res = invoke_func verbosity hs (s, Extract.empty_frame) args modname funcname fuel in 
+    let* res = invoke_func verbosity hs (s, Extract.empty_frame) args modname funcname max_call_depth in 
       debug_info verbosity stage (fun _ -> "Successfully executed function " ^ funcname ^ " of module: " ^ modname ^ ".\n");
       pure res
 
@@ -192,7 +192,7 @@ type verdict_detail =
   | Verdict_OK
   | Verdict_inst_trap
 
-let run_wast_command verbosity timeout fuel cmd hs s mod_counter default_module_name test_counter =
+let run_wast_command verbosity timeout max_call_depth cmd hs s mod_counter default_module_name test_counter =
   debug_info verbosity stage 
   (fun _ -> 
     "\n\n----------\nTest " ^ string_of_int test_counter ^ "\n----------\n" ^ print_wast_command cmd ^ "\n"
@@ -210,7 +210,7 @@ let run_wast_command verbosity timeout fuel cmd hs s mod_counter default_module_
   | Action act ->
     begin match act.it with
     | Invoke (ovar, funcname_utf8, val_args) ->
-      let* res = run_invoke verbosity (ovar, funcname_utf8, val_args) hs s default_module_name fuel in 
+      let* res = run_invoke verbosity (ovar, funcname_utf8, val_args) hs s default_module_name max_call_depth in 
       begin match res with
       | Cfg_err -> error "Invocation error"
       | Cfg_trap _ -> error "Unexpected trap"
@@ -228,7 +228,7 @@ let run_wast_command verbosity timeout fuel cmd hs s mod_counter default_module_
     | AssertReturn (act, expect_rets) ->
       begin match act.it with
       | Invoke (ovar, funcname_utf8, val_args) ->
-        let* res = run_invoke verbosity (ovar, funcname_utf8, val_args) hs s default_module_name fuel in 
+        let* res = run_invoke verbosity (ovar, funcname_utf8, val_args) hs s default_module_name max_call_depth in 
         begin match res with
         | Cfg_err -> error "Invocation error"
         | Cfg_exhaustion -> error "Unexpected exhaustion"
@@ -257,7 +257,7 @@ let run_wast_command verbosity timeout fuel cmd hs s mod_counter default_module_
     | AssertTrap (act, _) ->
       begin match act.it with
       | Invoke (ovar, funcname_utf8, val_args) ->
-        let* res = run_invoke verbosity (ovar, funcname_utf8, val_args) hs s default_module_name fuel in
+        let* res = run_invoke verbosity (ovar, funcname_utf8, val_args) hs s default_module_name max_call_depth in
         begin match res with
         | Cfg_err -> error "Invocation error"
         | Cfg_exhaustion -> error "Unexpected exhaustion when trap is expected"
@@ -273,12 +273,7 @@ let run_wast_command verbosity timeout fuel cmd hs s mod_counter default_module_
     | AssertExhaustion (act, _) ->
       begin match act.it with
       | Invoke (ovar, funcname_utf8, val_args) ->
-        let* res = try 
-        (with_timeout (timeout - 1) (fun _ -> run_invoke verbosity (ovar, funcname_utf8, val_args) hs s default_module_name fuel)) 
-      with | Timeout ->
-        debug_info verbosity stage (fun _ -> "An assert_exhaustion assertion was halted due to timing out\n");
-          pure Cfg_exhaustion
-      in
+        let* res = run_invoke verbosity (ovar, funcname_utf8, val_args) hs s default_module_name max_call_depth in
         begin match res with
         | Cfg_err -> error "Invocation error"
         | Cfg_res _ ->
@@ -363,14 +358,14 @@ let run_wast_command verbosity timeout fuel cmd hs s mod_counter default_module_
 end
     
 
-let rec run_wast_commands verbosity timeout fuel cmds hs s mod_counter default_module_name assert_ok assert_total =
+let rec run_wast_commands verbosity timeout max_call_depth cmds hs s mod_counter default_module_name assert_ok assert_total =
   match cmds with
   | [] -> 
     pure (assert_ok, assert_total)
   | cmd :: cmds' ->
       let verdict = 
         try
-          (with_timeout timeout (fun _ -> run_wast_command verbosity timeout fuel cmd hs s mod_counter default_module_name (assert_total+1))) with
+          (with_timeout timeout (fun _ -> run_wast_command verbosity timeout max_call_depth cmd hs s mod_counter default_module_name (assert_total+1))) with
           | Timeout -> error "Execution was timed out"
          in
         begin match to_out verdict with
@@ -382,14 +377,14 @@ let rec run_wast_commands verbosity timeout fuel cmds hs s mod_counter default_m
             let new_total = assert_total + 1 in
               Printf.printf "\rTests passed: %d/%d (%.2f%%) " new_ok new_total (float_of_int new_ok *. 100.0 /. float_of_int new_total);
               flush stdout;
-              run_wast_commands verbosity timeout fuel cmds' hs' s' mod_counter' default_module_name' new_ok new_total
+              run_wast_commands verbosity timeout max_call_depth cmds' hs' s' mod_counter' default_module_name' new_ok new_total
           | Verdict_inst_trap ->
             let new_ok = assert_ok in
             let new_total = assert_total + 1 in
               debug_info verbosity stage (fun _ -> "Successfully loaded module, but post-instantiation initialisation trapped\n");
               Printf.printf "\rTests failed: %d/%d (%.2f%%) " new_ok new_total (float_of_int new_ok *. 100.0 /. float_of_int new_total);
               flush stdout;
-              run_wast_commands verbosity timeout fuel cmds' hs' s' mod_counter' default_module_name' new_ok new_total
+              run_wast_commands verbosity timeout max_call_depth cmds' hs' s' mod_counter' default_module_name' new_ok new_total
           end
         | Error msg ->
             debug_info verbosity stage ~style:red (fun _ -> "Test failed: " ^ msg ^ "\n");
@@ -397,7 +392,7 @@ let rec run_wast_commands verbosity timeout fuel cmds hs s mod_counter default_m
             let new_total = assert_total + 1 in
             Printf.printf "\rTests passed: %d/%d (%.2f%%) " new_ok new_total (float_of_int new_ok *. 100.0 /. float_of_int new_total);
             flush stdout;
-            run_wast_commands verbosity timeout fuel cmds' hs s mod_counter default_module_name new_ok new_total
+            run_wast_commands verbosity timeout max_call_depth cmds' hs s mod_counter default_module_name new_ok new_total
           end
       
 
@@ -429,11 +424,11 @@ let register_spectest_host verbosity hs s =
     debug_info verbosity stage (fun _ -> "Successfully instantiated module " ^ modname ^ ".\n");
     pure (hs', s')
 
-let run_wast_script verbosity timeout fuel script =
+let run_wast_script verbosity timeout max_call_depth script =
   let starting_host_store = (Execute.StringMap.empty, Execute.StringMap.empty) in
   let starting_store = empty_store_record in
   let* (hs, s) = register_spectest_host verbosity starting_host_store starting_store in
-  let* ret = run_wast_commands verbosity timeout fuel script hs s 0 "" 0 0 in
+  let* ret = run_wast_commands verbosity timeout max_call_depth script hs s 0 "" 0 0 in
   match ret with
     | (assert_ok, assert_total) -> 
       debug_info verbosity result (fun _ -> "\n");
@@ -442,9 +437,9 @@ let run_wast_script verbosity timeout fuel script =
       pure ()
     
 
-let run_wast_string verbosity timeout fuel scriptstr = 
+let run_wast_string verbosity timeout max_call_depth scriptstr = 
   let script = Parse.parse_wast scriptstr in
-  run_wast_script verbosity timeout fuel script
+  run_wast_script verbosity timeout max_call_depth script
 
 
   
